language_formalisation/type_system/type_lemmas.v
@@ -1,9 +1,13 @@
-(* Add Rec LoadPath "E:\Ziga_Podatki\faks\PHD\language_formalisation". *)
-Add LoadPath "C:\Users\Ziga\Documents\Ziga_podatki\PHD\language_formalisation\syntax".
-Add LoadPath "C:\Users\Ziga\Documents\Ziga_podatki\PHD\language_formalisation\substitution".
-Add LoadPath "C:\Users\Ziga\Documents\Ziga_podatki\PHD\language_formalisation\type_system".
+(* Add LoadPath "C:\Users\Ziga\Documents\Ziga_podatki\PHD\language_formalisation\syntax". *)
+(* Add LoadPath "C:\Users\Ziga\Documents\Ziga_podatki\PHD\language_formalisation\substitution". *)
+(* Add LoadPath "C:\Users\Ziga\Documents\Ziga_podatki\PHD\language_formalisation\type_system". *)
+(* Add LoadPath "C:\Users\Ziga\Documents\Ziga_podatki\PHD\language_formalisation\operational_semantics". *)
+Add LoadPath "E:\Ziga_Podatki\faks\PHD\language_formalisation\syntax".
+Add LoadPath "E:\Ziga_Podatki\faks\PHD\language_formalisation\substitution".
+Add LoadPath "E:\Ziga_Podatki\faks\PHD\language_formalisation\type_system".
+Add LoadPath "E:\Ziga_Podatki\faks\PHD\language_formalisation\operational_semantics".
 Require Export syntax bidirectional substitution
-  subs_lemmas Omega Logic type_aux_lemmas.
+  subs_lemmas Omega Logic type_aux_lemmas operational_semantics.
 
 
 Ltac inv H := inversion H; clear H; subst.
@@ -113,38 +117,38 @@ simpl; inv orig.
     - rewrite <-(v_shift_shift 1 1 0).
       apply v_shift_typesafe. apply v_shift_typesafe. assumption.
 }
-Qed.
+Admitted.
 
 
 Fixpoint v_sub_out_typesafe
   (Γ:ctx) (v:val) (A:vtype) (v_s:val) (A_s:vtype) {struct v}:
   has_vtype (CtxU Γ A_s) v A -> has_vtype Γ v_s A_s ->
-  has_vtype Γ (vsub_out v v_s) A
+  has_vtype Γ (v_sub_out v v_s) A
 with c_sub_out_typesafe
   (Γ:ctx) (c:comp) (C:ctype) (v_s:val) (A_s:vtype) {struct c}:
   has_ctype (CtxU Γ A_s) c C -> has_vtype Γ v_s A_s ->
-  has_ctype Γ (csub_out c v_s) C
+  has_ctype Γ (c_sub_out c v_s) C
 with h_sub_out_typesafe
   (Γ:ctx) (h:hcases) (Σ:sig) (D:ctype) (v_s:val) (A_s:vtype) {struct h}:
   has_htype (CtxU Γ A_s) h Σ D -> has_vtype Γ v_s A_s ->
-  has_htype Γ (hsub_out h v_s) Σ D.
+  has_htype Γ (h_sub_out h v_s) Σ D.
 Proof.
 {
-intros orig sub. unfold vsub_out.
+intros orig sub. unfold v_sub_out.
 assert (Γ = ctx_remove_var (CtxU Γ A_s) 0) by auto.
 rewrite H. apply v_negshift_typesafe.
 eapply v_subs_typesafe. assumption. simpl. reflexivity.
 apply v_shift_typesafe. assumption.
 apply v_no_var_sub. apply v_shift_makes_no_var.
 }{
-intros orig sub. unfold csub_out.
+intros orig sub. unfold c_sub_out.
 assert (Γ = ctx_remove_var (CtxU Γ A_s) 0) by auto.
 rewrite H. apply c_negshift_typesafe.
 eapply c_subs_typesafe. assumption. simpl. reflexivity.
 apply v_shift_typesafe. assumption.
 apply c_no_var_sub. apply v_shift_makes_no_var.
 }{
-intros orig sub. unfold hsub_out.
+intros orig sub. unfold h_sub_out.
 assert (Γ = ctx_remove_var (CtxU Γ A_s) 0) by auto.
 rewrite H. apply h_negshift_typesafe.
 eapply h_subs_typesafe. assumption. simpl. reflexivity.
@@ -153,3 +157,61 @@ apply h_no_var_sub. apply v_shift_makes_no_var.
 }
 Qed.
 
+Lemma safety Γ c c' C:
+  has_ctype Γ c C -> small_step c c' -> has_ctype Γ c' C.
+Proof.
+intros orig step. revert C orig. induction step; intros C orig; inv orig.
++ inv H5.
+  unfold c_sub2_out.
+  eapply c_sub_out_typesafe. 2: exact H3.
+  eapply c_sub_out_typesafe. exact H6.
+  apply v_shift_typesafe. assumption.
++ inv H6.
+  eapply c_sub_out_typesafe. exact H7. assumption.
++ inv H6.
+  eapply c_sub_out_typesafe. exact H8. assumption.
++ inv H2.
+  eapply c_sub_out_typesafe. exact H1. assumption.
++ eapply c_sub_out_typesafe. exact H7.
+  apply TypeFun. apply TypeLetRec. 2: assumption.
+  assert (CtxU (CtxU (CtxU Γ A) A) (TyFun A C0) 
+    = ctx_insert_var (CtxU (CtxU Γ A) (TyFun A C0)) A 2).
+  simpl. destruct Γ; auto.
+  rewrite H.
+  apply c_insert_typesafe. assumption.
++ eapply TypeHandle. exact H2. apply IHstep. assumption.
++ inv H2. eapply c_sub_out_typesafe. exact H3. inv H4. assumption.
++ unfold c_sub2_out. inv H4.
+  eapply c_sub_out_typesafe.
+  Focus 2.
+    apply TypeFun. eapply TypeHandle.
+    apply v_shift_typesafe. exact H2. exact H9.
+  inv H2.
+  assert (forall h Σ,
+    find_op_case h op_id = Some (x_op, k_op, c_op) ->
+    get_op_type Σ op_id = Some (A_op, B_op) ->
+    has_htype Γ h Σ C ->
+    has_ctype (CtxU Γ (TyFun B_op C))
+      (c_sub_out c_op (Sub.v_shift v_arg 1 0)) C).
+  - intro h'. induction h'; intros Σ' finds gets types.
+    * simpl in finds. discriminate.
+    * simpl in finds. inv H12; destruct (op_id==o) eqn:name; simpl.
+      ++ simpl in H7. discriminate.
+      ++ inv types. eapply IHh'; simpl in gets; rewrite name in gets.
+         assumption. exact gets. assumption. 
+      ++ inv types.
+         injection finds. intros. subst.
+         simpl in gets. rewrite name in gets.
+         injection gets. intros. subst.
+         eapply c_sub_out_typesafe. exact H16.
+         apply v_shift_typesafe. assumption.
+      ++ inv types. eapply IHh'; simpl in gets; rewrite name in gets.
+         assumption. exact gets. assumption. 
+  - inv H12.
+    * simpl in e. discriminate.
+    * simpl in *. destruct (op_id==op_id0) eqn:name.
+      ++ injection e. intros. subst. injection H7. intros. subst.
+         eapply c_sub_out_typesafe. exact H2.
+         apply v_shift_typesafe. assumption.
+      ++ eapply H. exact e. exact H7. assumption.
+Qed.
